common/Memtype.v
@@ -93,12 +93,13 @@ Parameter sup_In : block -> sup -> Prop.
 Parameter empty_in: forall b, ~ sup_In b sup_empty.
 Parameter sup_dec : forall b s, {sup_In b s}+{~sup_In b s}.
 
-Parameter fresh_block : sup -> block.
-Parameter freshness : forall s, ~sup_In (fresh_block s) s.
+Parameter info : Type.
+Parameter fresh_block : info -> sup -> block.
+Parameter freshness : forall i s, ~sup_In (fresh_block i s) s.
 
 Parameter sup_add : block -> sup -> sup.
 
-Definition sup_incr(s:sup) := sup_add (fresh_block s) s.
+Definition sup_incr(i:info)(s:sup) := sup_add (fresh_block i s) s.
 
 Definition sup_include(s1 s2:sup) := forall b, sup_In b s1 -> sup_In b s2.
 
@@ -145,7 +146,7 @@ Parameter empty: mem.
   Returns a pair [(m', b)] of the updated memory state [m'] and
   the identifier [b] of the newly-allocated block.
   Note that [alloc] never fails: we are modeling an infinite memory. *)
-Parameter alloc: forall (m: mem) (lo hi: Z), mem * block.
+Parameter alloc: forall (i:info)(m: mem) (lo hi: Z), mem * block.
 
 (** [free m b lo hi] frees (deallocates) the range of offsets from [lo]
   included to [hi] excluded in block [b].  Returns the updated memory
@@ -219,7 +220,7 @@ Parameter drop_perm: forall (m: mem) (b: block) (lo hi: Z) (p: permission), opti
   block. *)
 
 Parameter support: mem -> sup.
-Parameter nextblock: mem -> block.
+Parameter nextblock: info -> mem -> block.
 
 Parameter valid_block: mem->block->Prop.
 
@@ -437,8 +438,8 @@ Axiom loadbytes_split:
   is valid for writing. *)
 
 Axiom nextblock_store:
-  forall chunk m1 b ofs v m2, store chunk m1 b ofs v = Some m2 ->
-  nextblock m2 = nextblock m1.
+  forall chunk m1 b ofs v m2 i, store chunk m1 b ofs v = Some m2 ->
+  nextblock i m2 = nextblock i m1.
 Axiom store_valid_block_1:
   forall chunk m1 b ofs v m2, store chunk m1 b ofs v = Some m2 ->
   forall b', valid_block m1 b' -> valid_block m2 b'.
@@ -585,8 +586,8 @@ Axiom storebytes_valid_access_2:
   forall chunk' b' ofs' p,
   valid_access m2 chunk' b' ofs' p -> valid_access m1 chunk' b' ofs' p.
 Axiom nextblock_storebytes:
-  forall m1 b ofs bytes m2, storebytes m1 b ofs bytes = Some m2 ->
-  nextblock m2 = nextblock m1.
+  forall m1 b ofs bytes m2 i, storebytes m1 b ofs bytes = Some m2 ->
+  nextblock i m2 = nextblock i m1.
 Axiom storebytes_valid_block_1:
   forall m1 b ofs bytes m2, storebytes m1 b ofs bytes = Some m2 ->
   forall b', valid_block m1 b' -> valid_block m2 b'.
@@ -648,8 +649,8 @@ Axiom storebytes_split:
   of the initial memory state. *)
 
 Axiom alloc_result:
-  forall m1 lo hi m2 b, alloc m1 lo hi = (m2, b) ->
-  b = nextblock m1.
+  forall m1 lo hi m2 b i, alloc i m1 lo hi = (m2, b) ->
+  b = nextblock i m1.
 
 (** Effect of [alloc] on block validity. *)
 (*
@@ -658,34 +659,34 @@ Axiom nextblock_alloc:
   nextblock m2 = Pos.succ (nextblock m1).
 *)
 Axiom valid_block_alloc:
-  forall m1 lo hi m2 b, alloc m1 lo hi = (m2, b) ->
+  forall m1 lo hi m2 b i, alloc i m1 lo hi = (m2, b) ->
   forall b', valid_block m1 b' -> valid_block m2 b'.
 Axiom fresh_block_alloc:
-  forall m1 lo hi m2 b, alloc m1 lo hi = (m2, b) ->
+  forall m1 lo hi m2 b i, alloc i m1 lo hi = (m2, b) ->
   ~(valid_block m1 b).
 Axiom valid_new_block:
-  forall m1 lo hi m2 b, alloc m1 lo hi = (m2, b) ->
+  forall m1 lo hi m2 b i, alloc i m1 lo hi = (m2, b) ->
   valid_block m2 b.
 Axiom valid_block_alloc_inv:
-  forall m1 lo hi m2 b, alloc m1 lo hi = (m2, b) ->
+  forall m1 lo hi m2 b i, alloc i m1 lo hi = (m2, b) ->
   forall b', valid_block m2 b' -> b' = b \/ valid_block m1 b'.
 
 (** Effect of [alloc] on permissions. *)
 
 Axiom perm_alloc_1:
-  forall m1 lo hi m2 b, alloc m1 lo hi = (m2, b) ->
+  forall m1 lo hi m2 b i, alloc i m1 lo hi = (m2, b) ->
   forall b' ofs k p, perm m1 b' ofs k p -> perm m2 b' ofs k p.
 Axiom perm_alloc_2:
-  forall m1 lo hi m2 b, alloc m1 lo hi = (m2, b) ->
+  forall m1 lo hi m2 b i, alloc i m1 lo hi = (m2, b) ->
   forall ofs k, lo <= ofs < hi -> perm m2 b ofs k Freeable.
 Axiom perm_alloc_3:
-  forall m1 lo hi m2 b, alloc m1 lo hi = (m2, b) ->
+  forall m1 lo hi m2 b i, alloc i m1 lo hi = (m2, b) ->
   forall ofs k p, perm m2 b ofs k p -> lo <= ofs < hi.
 Axiom perm_alloc_4:
-  forall m1 lo hi m2 b, alloc m1 lo hi = (m2, b) ->
+  forall m1 lo hi m2 b i, alloc i m1 lo hi = (m2, b) ->
   forall b' ofs k p, perm m2 b' ofs k p -> b' <> b -> perm m1 b' ofs k p.
 Axiom perm_alloc_inv:
-  forall m1 lo hi m2 b, alloc m1 lo hi = (m2, b) ->
+  forall m1 lo hi m2 b i, alloc i m1 lo hi = (m2, b) ->
   forall b' ofs k p,
   perm m2 b' ofs k p ->
   if eq_block b' b then lo <= ofs < hi else perm m1 b' ofs k p.
@@ -693,17 +694,17 @@ Axiom perm_alloc_inv:
 (** Effect of [alloc] on access validity. *)
 
 Axiom valid_access_alloc_other:
-  forall m1 lo hi m2 b, alloc m1 lo hi = (m2, b) ->
+  forall m1 lo hi m2 b i, alloc i m1 lo hi = (m2, b) ->
   forall chunk b' ofs p,
   valid_access m1 chunk b' ofs p ->
   valid_access m2 chunk b' ofs p.
 Axiom valid_access_alloc_same:
-  forall m1 lo hi m2 b, alloc m1 lo hi = (m2, b) ->
+  forall m1 lo hi m2 b i, alloc i m1 lo hi = (m2, b) ->
   forall chunk ofs,
   lo <= ofs -> ofs + size_chunk chunk <= hi -> (align_chunk chunk | ofs) ->
   valid_access m2 chunk b ofs Freeable.
 Axiom valid_access_alloc_inv:
-  forall m1 lo hi m2 b, alloc m1 lo hi = (m2, b) ->
+  forall m1 lo hi m2 b i, alloc i m1 lo hi = (m2, b) ->
   forall chunk b' ofs p,
   valid_access m2 chunk b' ofs p ->
   if eq_block b' b
@@ -713,22 +714,22 @@ Axiom valid_access_alloc_inv:
 (** Load-alloc properties. *)
 
 Axiom load_alloc_unchanged:
-  forall m1 lo hi m2 b, alloc m1 lo hi = (m2, b) ->
+  forall m1 lo hi m2 b i, alloc i m1 lo hi = (m2, b) ->
   forall chunk b' ofs,
   valid_block m1 b' ->
   load chunk m2 b' ofs = load chunk m1 b' ofs.
 Axiom load_alloc_other:
-  forall m1 lo hi m2 b, alloc m1 lo hi = (m2, b) ->
+  forall m1 lo hi m2 b i, alloc i m1 lo hi = (m2, b) ->
   forall chunk b' ofs v,
   load chunk m1 b' ofs = Some v ->
   load chunk m2 b' ofs = Some v.
 Axiom load_alloc_same:
-  forall m1 lo hi m2 b, alloc m1 lo hi = (m2, b) ->
+  forall m1 lo hi m2 b i, alloc i m1 lo hi = (m2, b) ->
   forall chunk ofs v,
   load chunk m2 b ofs = Some v ->
   v = Vundef.
 Axiom load_alloc_same':
-  forall m1 lo hi m2 b, alloc m1 lo hi = (m2, b) ->
+  forall m1 lo hi m2 b i, alloc i m1 lo hi = (m2, b) ->
   forall chunk ofs,
   lo <= ofs -> ofs + size_chunk chunk <= hi -> (align_chunk chunk | ofs) ->
   load chunk m2 b ofs = Some Vundef.
@@ -748,9 +749,9 @@ Axiom free_range_perm:
 
 (** Block validity is preserved by [free]. *)
 
-Axiom nextblock_free:
-  forall m1 bf lo hi m2, free m1 bf lo hi = Some m2 ->
-  nextblock m2 = nextblock m1.
+Axiom support_free:
+  forall m1 bf lo hi m2 , free m1 bf lo hi = Some m2 ->
+  support m2 = support m1.
 Axiom valid_block_free_1:
   forall m1 bf lo hi m2, free m1 bf lo hi = Some m2 ->
   forall b, valid_block m1 b -> valid_block m2 b.
@@ -808,9 +809,9 @@ Axiom load_free:
 
 (** ** Properties of [drop_perm]. *)
 
-Axiom nextblock_drop:
+Axiom support_drop:
   forall m b lo hi p m', drop_perm m b lo hi p = Some m' ->
-  nextblock m' = nextblock m.
+  support m' = support m.
 Axiom drop_perm_valid_block_1:
   forall m b lo hi p m', drop_perm m b lo hi p = Some m' ->
   forall b', valid_block m b' -> valid_block m' b'.
@@ -921,12 +922,12 @@ Axiom storebytes_outside_extends:
   extends m1 m2'.
 
 Axiom alloc_extends:
-  forall m1 m2 lo1 hi1 b m1' lo2 hi2,
+  forall m1 m2 lo1 hi1 b m1' lo2 hi2 i,
   extends m1 m2 ->
-  alloc m1 lo1 hi1 = (m1', b) ->
+  alloc i m1 lo1 hi1 = (m1', b) ->
   lo2 <= lo1 -> hi1 <= hi2 ->
   exists m2',
-     alloc m2 lo2 hi2 = (m2', b)
+     alloc i m2 lo2 hi2 = (m2', b)
   /\ extends m1' m2'.
 
 Axiom free_left_extends:
@@ -1168,15 +1169,15 @@ Axiom storebytes_outside_inject:
   inject f m1 m2'.
 
 Axiom alloc_right_inject:
-  forall f m1 m2 lo hi b2 m2',
+  forall f m1 m2 lo hi b2 m2' i,
   inject f m1 m2 ->
-  alloc m2 lo hi = (m2', b2) ->
+  alloc i m2 lo hi = (m2', b2) ->
   inject f m1 m2'.
 
 Axiom alloc_left_unmapped_inject:
-  forall f m1 m2 lo hi m1' b1,
+  forall f m1 m2 lo hi m1' b1 i,
   inject f m1 m2 ->
-  alloc m1 lo hi = (m1', b1) ->
+  alloc i m1 lo hi = (m1', b1) ->
   exists f',
      inject f' m1' m2
   /\ inject_incr f f'
@@ -1187,9 +1188,9 @@ Definition inj_offset_aligned (delta: Z) (size: Z) : Prop :=
   forall chunk, size_chunk chunk <= size -> (align_chunk chunk | delta).
 
 Axiom alloc_left_mapped_inject:
-  forall f m1 m2 lo hi m1' b1 b2 delta,
+  forall f m1 m2 lo hi m1' b1 b2 delta i,
   inject f m1 m2 ->
-  alloc m1 lo hi = (m1', b1) ->
+  alloc i m1 lo hi = (m1', b1) ->
   valid_block m2 b2 ->
   0 <= delta <= Ptrofs.max_unsigned ->
   (forall ofs k p, perm m2 b2 ofs k p -> delta = 0 \/ 0 <= ofs < Ptrofs.max_unsigned) ->
@@ -1206,12 +1207,12 @@ Axiom alloc_left_mapped_inject:
   /\ (forall b, b <> b1 -> f' b = f b).
 
 Axiom alloc_parallel_inject:
-  forall f m1 m2 lo1 hi1 m1' b1 lo2 hi2,
+  forall f m1 m2 lo1 hi1 m1' b1 lo2 hi2 i,
   inject f m1 m2 ->
-  alloc m1 lo1 hi1 = (m1', b1) ->
+  alloc i m1 lo1 hi1 = (m1', b1) ->
   lo2 <= lo1 -> hi1 <= hi2 ->
   exists f', exists m2', exists b2,
-  alloc m2 lo2 hi2 = (m2', b2)
+  alloc i m2 lo2 hi2 = (m2', b2)
   /\ inject f' m1' m2'
   /\ inject_incr f f'
   /\ f' b1 = Some(b2, 0)
@@ -1260,8 +1261,8 @@ Axiom empty_inject_neutral:
   forall s, inject_neutral s empty.
 
 Axiom alloc_inject_neutral:
-  forall s m lo hi b m',
-  alloc m lo hi = (m', b) ->
+  forall s m lo hi b m' i,
+  alloc i m lo hi = (m', b) ->
   inject_neutral s m ->
   sup_include (sup_add b (support m)) s ->
   inject_neutral s m'.
