common/Values.v
@@ -20,7 +20,6 @@ Require Import Coqlib.
 Require Import AST.
 Require Import Integers.
 Require Import Floats.
-
 Module Type BLOCK.
 
 Parameter block : Type.
@@ -30,14 +29,63 @@ End BLOCK.
 
 (* Declare Module Block : BLOCK. *)
 
+(*
 Module Block <: BLOCK.
 Definition block := positive.
 Definition eq_block := peq.
+End Block.
+*)
+Inductive block' :=
+  |Stack : positive -> block'
+  |Other : positive -> block'.
+
+Module Block <: BLOCK.
+
+Definition block := block'.
+
+Theorem eq_block : forall (x y:block),{x=y}+{x<>y}.
+Proof.
+  intros. destruct x; destruct y; try (right; discriminate);
+  destruct (peq p p0); try (left; rewrite e; auto); right; congruence.
+(*
+  intros. destruct x; destruct y. destruct (list_eq_dec peq l l0).
+  left. rewrite e. auto. right. congruence.
+  right. discriminate. right. discriminate.
+  destruct (peq p p0). left. rewrite e. auto.
+  right. congruence.
+*)
+Qed.
+
 End Block.
 
 Definition block := Block.block.
 Definition eq_block := Block.eq_block.
 
+
+Definition posb (b:block) : positive :=
+  match b with
+    | Stack p => p
+    | Other p => p
+  end.
+(*
+Definition listb (b:block) : option (list positive) :=
+  match b with
+    | Stack l => Some l
+    | Other _ => None
+  end.
+*)
+
+Definition succ (b:block) : block :=
+  match b with
+    | Stack p => Stack (Pos.succ p)
+    | Other p => Other (Pos.succ p)
+  end.
+
+Definition is_stack (b:block) : bool :=
+  match b with
+    | Stack _ => true
+    |  _ => false
+  end.
 
 (** A value is either:
 - a machine integer;
