common/Separation.v
@@ -331,8 +331,8 @@ Next Obligation.
 Qed.
 
 Lemma alloc_rule:
-  forall m lo hi b m' P,
-  Mem.alloc m lo hi = (m', b) ->
+  forall m lo hi b m' P i,
+  Mem.alloc i m lo hi = (m', b) ->
   0 <= lo -> hi <= Ptrofs.modulus ->
   m |= P ->
   m' |= range b lo hi ** P.
@@ -674,10 +674,10 @@ Proof.
 Qed.
 
 Lemma alloc_parallel_rule:
-  forall m1 sz1 m1' b1 m2 sz2 m2' b2 P j lo hi delta,
+  forall m1 sz1 m1' b1 m2 sz2 m2' b2 P j lo hi delta i,
   m2 |= minjection j m1 ** P ->
-  Mem.alloc m1 0 sz1 = (m1', b1) ->
-  Mem.alloc m2 0 sz2 = (m2', b2) ->
+  Mem.alloc i m1 0 sz1 = (m1', b1) ->
+  Mem.alloc i m2 0 sz2 = (m2', b2) ->
   (8 | delta) ->
   lo = delta ->
   hi = delta + Z.max 0 sz1 ->
@@ -689,7 +689,7 @@ Lemma alloc_parallel_rule:
   /\ j' b1 = Some(b2, delta)
   /\ (forall b, b <> b1 -> j' b = j b).
 Proof.
-  intros until delta; intros SEP ALLOC1 ALLOC2 ALIGN LO HI RANGE1 RANGE2 RANGE3.
+  intros until delta; intros i SEP ALLOC1 ALLOC2 ALIGN LO HI RANGE1 RANGE2 RANGE3.
   assert (RANGE4: lo <= hi) by extlia.
   assert (FRESH1: ~Mem.valid_block m1 b1) by (eapply Mem.fresh_block_alloc; eauto).
   assert (FRESH2: ~Mem.valid_block m2 b2) by (eapply Mem.fresh_block_alloc; eauto).
@@ -884,10 +884,10 @@ Proof.
 Qed.
 
 Lemma alloc_parallel_rule_2:
-  forall (F V: Type) (ge: Genv.t F V) m1 sz1 m1' b1 m2 sz2 m2' b2 P j lo hi delta,
+  forall (F V: Type) (ge: Genv.t F V) m1 sz1 m1' b1 m2 sz2 m2' b2 P j lo hi delta i,
   m2 |= minjection j m1 ** globalenv_inject ge j ** P ->
-  Mem.alloc m1 0 sz1 = (m1', b1) ->
-  Mem.alloc m2 0 sz2 = (m2', b2) ->
+  Mem.alloc i m1 0 sz1 = (m1', b1) ->
+  Mem.alloc i m2 0 sz2 = (m2', b2) ->
   (8 | delta) ->
   lo = delta ->
   hi = delta + Z.max 0 sz1 ->
